add in some reachable addr lemma

Splinter/Betree/Branches.i.dfy
@@ -26,7 +26,14 @@ module BranchesMod {
 			&& (forall root | root in roots :: diskView.ValidAddress(root))
       && (forall root | root in roots :: GetBranch(root).Acyclic())
       && (forall root | root in roots :: GetBranch(root).AllKeysInRange())
+      && BranchesDisjoint()
 		}
+
+    predicate BranchesDisjoint()
+    {
+      && (forall r1, r2 | r1 in roots && r2 in roots && r1 != r2 :: 
+        GetBranch(r1).ReachableAddrs() !! GetBranch(r2).ReachableAddrs())
+    }
 
 		predicate ValidBranch(addr: Address)
 		{
@@ -36,7 +43,7 @@ module BranchesMod {
 		function GetBranch(addr: Address) : (branch: LinkedBranch)
       requires ValidBranch(addr)
 		{
-			LinkedBranch(addr, diskView)
+      LinkedBranch(addr, diskView)
 		}
 
 		function Query(key: Key, buffers: seq<Address>) : Message
@@ -51,21 +58,153 @@ module BranchesMod {
 			)
 		}
 
-    function AddBranch(branch: LinkedBranch) : Branches
+    function AddBranch(branch: LinkedBranch) : (out: Branches)
       requires WF()
       requires branch.Acyclic()
+      requires branch.AllKeysInRange()
       requires branch.TightDiskView()
       requires diskView.IsFresh(branch.ReachableAddrs())
     {
       Branches(roots + {branch.root}, diskView.MergeDisk(branch.diskView))
     }
     
-    function RemoveBranch(root: Address) : Branches
+    function RemoveBranch(root: Address) : (out: Branches)
       requires WF()
       requires ValidBranch(root)
     {
       var branchDisk := DiskView(MapRestrict(diskView.entries, GetBranch(root).ReachableAddrs()));
       Branches(roots - {root}, diskView.RemoveDisk(branchDisk))
+    }
+
+    // TODO: why we needed this again lol we will see if we can use it for 
+    // ah it's easier to put things togther this way I think
+    // like a compose rankings thing
+    function GetTightBranch(addr: Address) : (branch: LinkedBranch)
+      requires WF()
+      requires ValidBranch(addr)
+      ensures branch.WF()
+      ensures branch.Acyclic()
+    {
+      var branch := GetBranch(addr);
+      var tightDisk := DiskView(MapRestrict(diskView.entries, branch.ReachableAddrs()));
+      var tightBranch := LinkedBranch(addr, tightDisk);
+
+      assert tightDisk.WF() by {
+        forall addr | addr in tightDisk.entries 
+          ensures tightDisk.NodeHasValidChildAddress(tightDisk.entries[addr])
+        {
+          branch.ReachableAddrClosed(branch.TheRanking(), addr);
+        }
+      }
+
+      assert tightBranch.Acyclic() by {
+        assert tightBranch.ValidRanking(branch.TheRanking());
+      }
+
+      tightBranch
+    }
+
+    lemma AddBranchWF(branch: LinkedBranch) 
+      requires AddBranch.requires(branch)
+      ensures AddBranch(branch).WF()
+    {
+      // see if this can help us
+      // GetTightBranch
+
+      // assert (exists ranking | (forall r | r in roots :: MapsAgree(ranking, GetBranch(r).))
+      
+      
+      
+      // )
+      // var  := AddBranch(branch);
+
+      
+
+      // let's merge it 
+      // var ranking :| (forall r | r in roots :: MapsAgree(ranking, GetBranch(r).TheRanking()));
+      
+      // GetBranch(r).ValidRanking(ranking));
+      //diskView.ValidRanking(ranking) && (forall r | r in roots :: r in ranking); 
+
+
+      assume false;
+
+      // forall addr | addr in ranking 
+      //   && addr in entries 
+
+
+
+
+      //  assert forall addr | addr in diskView.entries :: 
+      //       && addr in newBranches.diskView.entries 
+      //       && diskView.entries[addr] == newBranches.diskView.entries[addr];
+      // assert newBranches.diskView.WF();
+      // var newRanking := 
+
+      // forall root | root in newBranches.roots
+      //   ensures newBranches.GetBranch(root).Acyclic()
+      // {
+        // maybe before this step what we want to prove is that 
+        // ValidRanking
+
+
+        // is it easier if I show that each is disjoint?
+        // maybe I am dying percisely bc I don't have a disjoint clause
+        
+      //   if root == branch.root {
+      //     assume false;
+      //   } else {
+      //     var b := GetBranch(root);
+      //     var b' := newBranches.GetBranch(root);
+
+      //     var ranking := b.TheRanking();
+      //     assert b.ValidRanking(ranking);
+      //     assert b.diskView == diskView;
+
+      //     // valid ranking 
+      //     // assert forall r | r in ranking :: r in diskView.entries 
+    
+      //     forall addr | addr in ranking && addr in newBranches.diskView.entries 
+      //       ensures newBranches.diskView.NodeChildrenRespectsRank(ranking, addr)
+      //     {
+      //       assert addr in diskView.entries;
+      //       // if addr in diskView.entries 
+          
+      //       // assert diskView.NodeChildrenRespectsRank(ranking, addr);
+      //       assume false;
+      //     }
+
+
+        
+
+      //     assert b'.ValidRanking(ranking);
+      //     assert b'.Acyclic();
+          
+
+
+      //     assume false;
+
+      //     assert newBranches.GetBranch(root).ValidRanking(GetBranch(root).TheRanking());
+      //     assert newBranches.GetBranch(root).Acyclic();
+      //     // GetBranch()
+      //   }
+
+      //   // assume false;
+      // }
+
+      // forall root | root in newBranches.roots
+      //   ensures newBranches.GetBranch(root).AllKeysInRange()
+      // {
+      //   assume false;
+      // }
+    }
+     
+     lemma RemoveBranchWF(root: Address) 
+      requires RemoveBranch.requires(root)
+      ensures RemoveBranch(root).WF() 
+    {
+      assume false;
+
     }
 	}
 }
