Splinter/Betree/LinkedBranch.i.dfy
@@ -316,6 +316,49 @@ module LinkedBranchMod {
         UnionSeqOfSetsSoundness(subTreeAddrs);
         {root} + UnionSeqOfSets(subTreeAddrs)
     }
+  
+    // TODO(Jialin): move to refinement instead?
+    // linked's children are always in the reachable set
+    lemma ChildrenAreReachable(ranking: Ranking)
+      requires WF()
+      requires Root().Index?
+      requires ValidRanking(ranking)
+      ensures forall i | 0 <= i < |Root().children| :: Root().children[i] in ReachableAddrsUsingRanking(ranking)
+    {
+      var numChildren := |Root().children|;
+      var subTreeAddrs := seq(numChildren, i requires 0 <= i < numChildren => ChildAtIdx(i).ReachableAddrsUsingRanking(ranking));
+
+      forall i | 0 <= i < numChildren  
+      ensures Root().children[i] in ReachableAddrsUsingRanking(ranking)
+      {
+        assert  Root().children[i] in subTreeAddrs[i];
+      }
+    }
+
+    // TODO(Jialin): move to refinement instead?
+    lemma ReachableAddrClosed(ranking: Ranking, addr: Address)
+      requires WF()
+      requires ValidRanking(ranking)
+      requires addr in ReachableAddrsUsingRanking(ranking)
+      ensures 
+        var node := diskView.entries[addr];
+        && (node.Index? ==> (forall i | 0 <= i < |node.children| :: node.children[i] in ReachableAddrsUsingRanking(ranking)))
+      decreases GetRank(ranking)
+    {
+      var node := diskView.entries[addr];
+
+      if node.Index? {
+        if addr == root {
+          ChildrenAreReachable(ranking);
+        } else {
+          var numChildren := |Root().children|;
+          var subTreeAddrs := seq(numChildren, i requires 0 <= i < numChildren => ChildAtIdx(i).ReachableAddrsUsingRanking(ranking));
+          UnionSeqOfSetsSoundness(subTreeAddrs);
+          var k :| 0 <= k < numChildren && addr in subTreeAddrs[k];
+          ChildAtIdx(k).ReachableAddrClosed(ranking, addr);
+        }
+      }
+    }
 
     predicate TightDiskView()
     {
